Capless/Subst/Term/Subcapturing.lean
@@ -9,76 +9,46 @@ Substitution theorems for term variable substitution in subcapturing judgments.
 
 namespace Capless
 
-mutual
 theorem CaptureKind.subst
   (h : CaptureKind Γ C K)
   (σ : VarSubst Γ f Δ) :
-  CaptureKind Δ (C.rename f) K :=
-  match h with
-  | .label hl =>
-    have hl1 := σ.lmap _ _ hl
-    .label hl1
-  | .cvar hb => by
-    have hb1 := σ.cmap _ _ hb
-    simp [CBinding.rename, CBound.rename] at hb1
-    apply CaptureKind.cvar hb1
-  | .csub hsub hk =>
-    have hsub1 := hsub.subst σ
-    .csub hsub1 (hk.subst σ)
-  | .sub hs hk => .sub hs (hk.subst σ)
-  | .empty => .empty
-  | .proj_kind => by
-    simp
-    apply CaptureKind.proj_kind
-  | .proj hk => by
-    simp
-    apply CaptureKind.proj $ hk.subst σ
-
+  CaptureKind Δ (C.rename f) K := by
+  induction h
+  case var hb hk ih =>
+    rewrite [CaptureSet.proj_rename] at ih
+    have h1 := Typing.inv_subcapt $ σ.map _ _ hb
+    apply subcapt $ ih σ
+    apply h1.apply_proj_singleton
+  case label hb => apply label (σ.lmap _ _ _ hb)
+  case cvar hb => apply cvar (σ.cmap _ _ hb)
+  case cbound hb hk ih =>
+    rewrite [CaptureSet.proj_rename] at ih
+    apply! cbound (σ.cmap _ _ hb) (ih _)
+  case cinstr hb hk ih =>
+    rewrite [CaptureSet.proj_rename] at ih
+    apply! cinstr (σ.cmap _ _ hb) (ih _)
+  case sub hs hk ih =>
+    apply! sub hs (ih _)
+  case empty => apply empty
+  case absurd he => apply! absurd
+  case union ha hb => apply! union (ha _) (hb _)
 
 theorem Subcapt.subst
   (h : Subcapt Γ C1 C2)
   (σ : VarSubst Γ f Δ) :
-  Subcapt Δ (C1.rename f) (C2.rename f) :=
-  match h with
-  | .trans ha hb => .trans (ha.subst σ) (hb.subst σ)
-  | .subset hsub => by
-    apply Subcapt.subset
-    apply CaptureSet.Subset.rename hsub
-  | .union h1 h2 => by
-    have ih1 := h1.subst σ
-    have ih2 := h2.subst σ
-    rw [CaptureSet.rename_union]
-    apply Subcapt.union <;> trivial
-  | .var hb => by
-    have ht := σ.map _ _ hb
-    simp [CType.rename] at ht
-    have h := Typing.inv_subcapt ht
-    trivial
-  | .cinstl hb =>
-    have hb1 := σ.cmap _ _ hb
-    .cinstl hb1
-  | .cinstr hb =>
-    have hb1 := σ.cmap _ _ hb
-    .cinstr hb1
-  | .cbound hb => by
-    have hb1 := σ.cmap _ _ hb
-    simp [CBinding.rename, CBound.rename] at hb1
-    apply Subcapt.cbound hb1
-  | .proj h1 => by
-    simp
-    apply Subcapt.proj (h1.subst σ)
-  | .proj_sub hs => by
-    simp
-    apply Subcapt.proj_sub hs
-  | .proj_l => by
-    simp
-    apply Subcapt.proj_l
-  | .proj_r hk => by
-    simp
-    apply Subcapt.proj_r (hk.subst σ)
-  | .proj_disj hd hk => by
-    simp
-    apply Subcapt.proj_disj hd (hk.subst σ)
-end
+  Subcapt Δ (C1.rename f) (C2.rename f) := by
+  induction h <;> try rw [CaptureSet.proj_rename]
+  case trans ha hb => apply! trans (ha _) (hb _)
+  case subset hs => apply subset (CaptureSet.Subset.rename hs)
+  case union ha hb => apply! union (ha _) (hb _)
+  case var hb =>
+    have h1 := Typing.inv_subcapt (σ.map _ _ hb)
+    apply h1.apply_proj_singleton
+  case cinstl hb => apply cinstl (σ.cmap _ _ hb)
+  case cinstr hb => apply cinstr (σ.cmap _ _ hb)
+  case cbound hb => apply cbound (σ.cmap _ _ hb)
+  case subkind hs => apply! subkind
+  case proj_absurd => apply! proj_absurd
+  case proj_split => apply! proj_split
 
 end Capless
